preliminary

src/Std/Tactic/BVDecide/Bitblast/BVExpr/Circuit/Impl/Substructure.lean
@@ -18,31 +18,79 @@ open Std.Sat Std.Sat.AIG
 
 namespace BVLogicalExpr
 
+structure Cache (aig : AIG BVBit) where
+  map : Std.HashMap BVLogicalExpr (Nat × Bool)
+  hbound : ∀ k (h : k ∈ map), (map.get k h).1 < aig.decls.size
+
+@[inline]
+def Cache.empty : Cache aig :=
+  ⟨{}, by simp⟩
+
+@[inline]
+def Cache.insert (cache : Cache aig) (expr : BVLogicalExpr) (ref : AIG.Ref aig) :
+    Cache aig :=
+  let ⟨map, hbound⟩ := cache
+  have := by sorry
+  ⟨map.insert expr ⟨ref.gate, ref.invert⟩, this⟩
+
+@[inline]
+def Cache.get? (cache : Cache aig) (expr : BVLogicalExpr) : Option (AIG.Ref aig) :=
+  match h : cache.map.get? expr with
+  | some ref =>
+    some ⟨ref.1, ref.2, sorry⟩
+  | none =>
+    none
+
+@[inline]
+def Cache.cast (cache : Cache aig1) (h : aig1.decls.size ≤ aig2.decls.size) :
+    Cache aig2 :=
+  let ⟨map, hbound⟩ := cache
+  have := by sorry
+  ⟨map, this⟩
+
+structure Return (aig : AIG BVBit) where
+  result : AIG.ExtendingEntrypoint aig
+  bvCache : BVExpr.Cache result.val.aig
+  logCache : Cache result.val.aig
+
 /--
 Turn a `BVLogicalExpr` into an `Entrypoint`.
 -/
 def bitblast (expr : BVLogicalExpr) : Entrypoint BVBit :=
-  go AIG.empty expr .empty |>.result.val
+  goCache AIG.empty expr .empty .empty |>.result.val
 where
-  go (aig : AIG BVBit) (expr : BVLogicalExpr) (cache : BVExpr.Cache aig) : Return aig :=
+  goCache (aig : AIG BVBit) (expr : BVLogicalExpr) (bvCache : BVExpr.Cache aig)
+      (logCache : Cache aig) : Return aig :=
+    match logCache.get? expr with
+    | some ref => ⟨⟨⟨aig, ref⟩, Nat.le_refl ..⟩, bvCache, logCache⟩
+    | none =>
+      let ⟨result, bvCache, logCache⟩ := go aig expr bvCache logCache
+      ⟨result, bvCache, logCache.insert expr result.val.ref⟩
+    termination_by (sizeOf expr, 1)
+
+  go (aig : AIG BVBit) (expr : BVLogicalExpr) (bvCache : BVExpr.Cache aig) (logCache : Cache aig) :
+      Return aig :=
     match expr with
-    | .atom pred => BVPred.bitblast aig ⟨pred, cache⟩
+    | .atom pred =>
+      let ⟨result, bvCache⟩ := BVPred.bitblast aig ⟨pred, bvCache⟩
+      ⟨result, bvCache, logCache.cast result.property⟩
     | .const val =>
       have := LawfulOperator.le_size (f := mkConstCached) ..
-      ⟨⟨aig.mkConstCached val, this⟩, cache.cast this⟩
+      ⟨⟨aig.mkConstCached val, this⟩, bvCache.cast this, logCache.cast this⟩
     | .not expr =>
-      let ⟨⟨⟨aig, exprRef⟩, hexpr⟩, cache⟩ := go aig expr cache
+      let ⟨⟨⟨aig, exprRef⟩, hexpr⟩, bvCache, logCache⟩ := goCache aig expr bvCache logCache
       let ret := aig.mkNotCached exprRef
       have := LawfulOperator.le_size (f := mkNotCached) ..
-      let cache := cache.cast this
+      let bvCache := bvCache.cast this
+      let logCache := logCache.cast this
       have := by
         apply LawfulOperator.le_size_of_le_aig_size (f := mkNotCached)
         exact hexpr
-      ⟨⟨ret, this⟩, cache⟩
+      ⟨⟨ret, this⟩, bvCache, logCache⟩
     | .ite discr lhs rhs =>
-      let ⟨⟨⟨aig, discrRef⟩, dextend⟩, cache⟩ := go aig discr cache
-      let ⟨⟨⟨aig, lhsRef⟩, lextend⟩, cache⟩ := go aig lhs cache
-      let ⟨⟨⟨aig, rhsRef⟩, rextend⟩, cache⟩ := go aig rhs cache
+      let ⟨⟨⟨aig, discrRef⟩, dextend⟩, bvCache, logCache⟩ := goCache aig discr bvCache logCache
+      let ⟨⟨⟨aig, lhsRef⟩, lextend⟩, bvCache, logCache⟩ := goCache aig lhs bvCache logCache
+      let ⟨⟨⟨aig, rhsRef⟩, rextend⟩, bvCache, logCache⟩ := goCache aig rhs bvCache logCache
       let discrRef := discrRef.cast <| by
         dsimp only at lextend rextend ⊢
         omega
@@ -53,15 +101,16 @@ where
       let input := ⟨discrRef, lhsRef, rhsRef⟩
       let ret := aig.mkIfCached input
       have := LawfulOperator.le_size (f := mkIfCached) ..
-      let cache := cache.cast this
+      let bvCache := bvCache.cast this
+      let logCache := logCache.cast this
       have := by
         apply LawfulOperator.le_size_of_le_aig_size (f := mkIfCached)
         dsimp only at dextend lextend rextend
         omega
-      ⟨⟨ret, this⟩, cache⟩
+      ⟨⟨ret, this⟩, bvCache, logCache⟩
     | .gate g lhs rhs =>
-      let ⟨⟨⟨aig, lhsRef⟩, lextend⟩, cache⟩ := go aig lhs cache
-      let ⟨⟨⟨aig, rhsRef⟩, rextend⟩, cache⟩ := go aig rhs cache
+      let ⟨⟨⟨aig, lhsRef⟩, lextend⟩, bvCache, logCache⟩ := goCache aig lhs bvCache logCache
+      let ⟨⟨⟨aig, rhsRef⟩, rextend⟩, bvCache, logCache⟩ := goCache aig rhs bvCache logCache
       let lhsRef := lhsRef.cast <| by
         dsimp only at rextend ⊢
         omega
@@ -70,55 +119,76 @@ where
       | .and =>
         let ret := aig.mkAndCached input
         have := LawfulOperator.le_size (f := mkAndCached) ..
-        let cache := cache.cast this
+        let bvCache := bvCache.cast this
+        let logCache := logCache.cast this
         have := by
           apply LawfulOperator.le_size_of_le_aig_size (f := mkAndCached)
           dsimp only at lextend rextend
           omega
-        ⟨⟨ret, this⟩, cache⟩
+        ⟨⟨ret, this⟩, bvCache, logCache⟩
       | .xor =>
         let ret := aig.mkXorCached input
         have := LawfulOperator.le_size (f := mkXorCached) ..
-        let cache := cache.cast this
+        let bvCache := bvCache.cast this
+        let logCache := logCache.cast this
         have := by
           apply LawfulOperator.le_size_of_le_aig_size (f := mkXorCached)
           dsimp only at lextend rextend
           omega
-        ⟨⟨ret, this⟩, cache⟩
+        ⟨⟨ret, this⟩, bvCache, logCache⟩
       | .beq =>
         let ret := aig.mkBEqCached input
         have := LawfulOperator.le_size (f := mkBEqCached) ..
-        let cache := cache.cast this
+        let bvCache := bvCache.cast this
+        let logCache := logCache.cast this
         have := by
           apply LawfulOperator.le_size_of_le_aig_size (f := mkBEqCached)
           dsimp only at lextend rextend
           omega
-        ⟨⟨ret, this⟩, cache⟩
+        ⟨⟨ret, this⟩, bvCache, logCache⟩
       | .or =>
         let ret := aig.mkOrCached input
         have := LawfulOperator.le_size (f := mkOrCached) ..
-        let cache := cache.cast this
+        let bvCache := bvCache.cast this
+        let logCache := logCache.cast this
         have := by
           apply LawfulOperator.le_size_of_le_aig_size (f := mkOrCached)
           dsimp only at lextend rextend
           omega
-        ⟨⟨ret, this⟩, cache⟩
+        ⟨⟨ret, this⟩, bvCache, logCache⟩
+    termination_by (sizeOf expr, 0)
 
 namespace bitblast
 
-theorem go_le_size (aig : AIG BVBit) (expr : BVLogicalExpr) (cache : BVExpr.Cache aig) :
-    aig.decls.size ≤ (go aig expr cache).result.val.aig.decls.size :=
-  (go aig expr cache).result.property
+theorem goCache_le_size (aig : AIG BVBit) (expr : BVLogicalExpr) (bvCache : BVExpr.Cache aig)
+    (logCache : Cache aig) :
+    aig.decls.size ≤ (goCache aig expr bvCache logCache).result.val.aig.decls.size :=
+  (goCache aig expr bvCache logCache).result.property
+
+theorem go_le_size (aig : AIG BVBit) (expr : BVLogicalExpr) (bvCache : BVExpr.Cache aig)
+    (logCache : Cache aig) :
+    aig.decls.size ≤ (go aig expr bvCache logCache).result.val.aig.decls.size :=
+  (go aig expr bvCache logCache).result.property
 
 theorem go_lt_size_of_lt_aig_size (aig : AIG BVBit) (expr : BVLogicalExpr)
-    (cache : BVExpr.Cache aig) (h : x < aig.decls.size) :
-    x < (go aig expr cache).result.val.aig.decls.size := by
+    (bvCache : BVExpr.Cache aig) (logCache : Cache aig) (h : x < aig.decls.size) :
+    x < (go aig expr bvCache logCache).result.val.aig.decls.size := by
   apply Nat.lt_of_lt_of_le
   · exact h
   · apply go_le_size
 
-theorem go_decl_eq (idx) (aig : AIG BVBit) (cache : BVExpr.Cache aig) (h : idx < aig.decls.size) (hbounds) :
-    (go aig expr cache).result.val.aig.decls[idx]'hbounds = aig.decls[idx] := by
+mutual
+
+theorem goCache_decl_eq (idx) (aig : AIG BVBit) (bvCache : BVExpr.Cache aig)
+    (logCache : Cache aig) (h : idx < aig.decls.size) (hbounds) :
+    (goCache aig expr bvCache logCache).result.val.aig.decls[idx]'hbounds = aig.decls[idx] := by
+  sorry
+
+theorem go_decl_eq (idx) (aig : AIG BVBit) (bvCache : BVExpr.Cache aig)
+    (logCache : Cache aig) (h : idx < aig.decls.size) (hbounds) :
+    (go aig expr bvCache logCache).result.val.aig.decls[idx]'hbounds = aig.decls[idx] := by
+  sorry
+  /-
   induction expr generalizing aig with
   | const =>
     simp only [go]
@@ -177,18 +247,30 @@ theorem go_decl_eq (idx) (aig : AIG BVBit) (cache : BVExpr.Cache aig) (h : idx <
         assumption
       · apply go_lt_size_of_lt_aig_size
         apply go_lt_size_of_lt_aig_size
-        assumption
+        assumption -/
 
-theorem go_isPrefix_aig {aig : AIG BVBit} (cache : BVExpr.Cache aig) :
-    IsPrefix aig.decls (go aig expr cache).result.val.aig.decls := by
+end
+
+theorem goCache_isPrefix_aig {aig : AIG BVBit} (bvCache : BVExpr.Cache aig)
+    (logCache : Cache aig) :
+    IsPrefix aig.decls (goCache aig expr bvCache logCache).result.val.aig.decls := by
+  apply IsPrefix.of
+  · intro idx h
+    apply goCache_decl_eq
+  · apply goCache_le_size
+
+theorem go_isPrefix_aig {aig : AIG BVBit} (bvCache : BVExpr.Cache aig)
+    (logCache : Cache aig) :
+    IsPrefix aig.decls (go aig expr bvCache logCache).result.val.aig.decls := by
   apply IsPrefix.of
   · intro idx h
     apply go_decl_eq
   · apply go_le_size
 
-theorem go_denote_mem_prefix (aig : AIG BVBit) (cache : BVExpr.Cache aig) (hstart) :
+theorem go_denote_mem_prefix (aig : AIG BVBit) (bvCache : BVExpr.Cache aig) (logCache : Cache aig)
+    (hstart) :
     ⟦
-      (go aig expr cache).result.val.aig,
+      (go aig expr bvCache logCache).result.val.aig,
       ⟨start, inv, go_lt_size_of_lt_aig_size (h := hstart) ..⟩,
       assign
     ⟧
